fixing assumption prover.

src/provers/AssumptionProver.v
@@ -1,83 +1,98 @@
-Require Import List.
-Require Import Expr Env.
-Require Import Prover ProverTac.
+Require Import ExtLib.Core.RelDec.
+Require Import ExtLib.Data.List.
+Require Import ExtLib.Tactics.Consider.
+Require Import MirrorCore.TypesI.
+Require Import MirrorCore.ExprI.
+Require Import MirrorCore.EnvI.
+Require Import MirrorCore.Prover.
+Require Import MirrorCore.provers.ProverTac.
+Require Import MirrorCore.ExprProp.
 
 Set Implicit Arguments.
 Set Strict Implicit.
 
-Local Notation "[ x , .. , y ]" := (cons x .. (cons y nil) ..).
-
 (** * The Assumption Prover **)
 
-Section AssumptionProver.
-  Variable types : list type.
-  Variable fs : functions types.
+Section proverI.
+  Context {typ : Type}.
+  Variable typD : list Type -> typ -> Type.
+  Context {RType_typ : RType typD}.
+  Variable expr : Type.
+  Context {Expr_expr : Expr typD expr}.
+  Context {typ0_prop : TypInstance0 typD Prop}.
+  Variable RD_expr : RelDec (@eq expr).
+  Variable RDC_expr : RelDec_Correct RD_expr.
+  Context {ExprOk_expr : ExprOk Expr_expr}.
 
-  Definition assumption_summary : Type := list (expr types).
+  Definition assumption_summary : Type := list expr.
 
-  Definition assumptionSummarize (hyps : list (expr types)) : assumption_summary := hyps.
+  Definition assumptionSummarize (hyps : list expr) : assumption_summary := hyps.
 
-  Fixpoint assumptionProve (hyps : assumption_summary)
-    (goal : expr types) : bool :=
-    match hyps with
-      | nil => false
-      | exp :: b => 
-        if expr_seq_dec exp goal
-        then true
-        else assumptionProve b goal
-    end.
+  Definition assumptionProve (hyps : assumption_summary)
+             (_ _ : tenv typ)
+             (goal : expr) : bool :=
+    anyb (rel_dec goal) hyps.
 
-  Definition assumptionLearn (sum : assumption_summary) (hyps : list (expr types)) : assumption_summary :=
-    sum ++ hyps.
+  Definition assumptionLearn (sum : assumption_summary) (hyps : list expr)
+  : assumption_summary :=
+    hyps ++ sum.
 
-  Definition assumptionValid (uvars vars : env types) (sum : assumption_summary) : Prop :=
-    AllProvable fs uvars vars sum.
+  Definition assumptionValid (uvars vars : env typD) (sum : assumption_summary)
+  : Prop :=
+    AllProvable typ0_prop uvars vars sum.
 
   Lemma assumptionValid_extensible : forall u g f ue ge,
     assumptionValid u g f -> assumptionValid (u ++ ue) (g ++ ge) f.
   Proof.
-    unfold assumptionValid. do 5 intro. eapply AllProvable_weaken.
+    unfold assumptionValid. do 5 intro.
+    eapply Forall_impl. intros. destruct H.
+    exists x. eapply exprD_weaken; eauto.
   Qed.
 
   Lemma assumptionSummarizeCorrect : forall uvars vars hyps,
-    AllProvable fs uvars vars hyps ->
+    AllProvable typ0_prop uvars vars hyps ->
     assumptionValid uvars vars (assumptionSummarize hyps).
+  Proof. auto. Qed.
+
+  Theorem Forall_app : forall T (P : T -> Prop) ls ls',
+    Forall P (ls ++ ls') <->
+    Forall P ls /\ Forall P ls'.
   Proof.
-    auto.
+    induction ls; simpl; split; try inversion 1; intros; subst; auto.
+    { apply IHls in H3. intuition. }
+    { intuition. inversion H2; subst. constructor; auto.
+      eapply IHls; intuition. }
   Qed.
 
   Lemma assumptionLearnCorrect : forall uvars vars sum,
-    assumptionValid uvars vars sum -> forall hyps, 
-    AllProvable fs uvars vars hyps ->
+    assumptionValid uvars vars sum -> forall hyps,
+    AllProvable typ0_prop uvars vars hyps ->
     assumptionValid uvars vars (assumptionLearn sum hyps).
   Proof.
     unfold assumptionLearn, assumptionValid. intuition.
-    apply AllProvable_app; auto.
+    apply Forall_app; auto.
   Qed.
 
-  Theorem assumptionProverCorrect : ProverCorrect fs assumptionValid assumptionProve.
-    t; induction sum; t; eauto.
+  Theorem assumptionProverCorrect : ProverCorrect assumptionValid assumptionProve.
+  Proof.
+    red. unfold assumptionValid, assumptionProve.
+    induction sum; simpl; intros; try congruence.
+    consider (goal ?[ eq ] a); intros; subst.
+    { inversion H; subst; auto. }
+    { inversion H; subst. intros. eauto. }
   Qed.
 
-  Definition assumptionProver : ProverT types :=
+  Definition assumptionProver : @ProverT typ expr :=
   {| Facts := assumption_summary
-   ; Summarize := assumptionSummarize
-   ; Learn := assumptionLearn
+   ; Summarize := fun _ _ => assumptionSummarize
+   ; Learn := fun f _ _ => assumptionLearn f
    ; Prove := assumptionProve
    |}.
-  Definition assumptionProver_correct : ProverT_correct (types := types) assumptionProver fs.
+
+  Definition assumptionProver_correct : ProverT_correct assumptionProver.
   eapply Build_ProverT_correct with (Valid := assumptionValid);
     eauto using assumptionValid_extensible, assumptionSummarizeCorrect, assumptionLearnCorrect, assumptionProverCorrect.
+  { simpl. intros. eapply assumptionLearnCorrect; eauto. }
   Qed.
 
-End AssumptionProver.
-
-(*
-Require Import Repr.
-
-Definition AssumptionProver : ProverPackage :=
-{| ProverTypes := nil_Repr EmptySet_type
- ; ProverFuncs := fun ts => nil_Repr (Default_signature ts)
- ; Prover_correct := fun ts fs => assumptionProver_correct fs
-|}.
-*)
+End proverI.
